simple/coq/Subtyping_inversion.v
@@ -2,9 +2,6 @@ Require Import Metalib.Metatheory.
 Require Import LibTactics.
 Require Import syntax_ott
                rules_inf.
-Require Import Omega.
-
-
 
 Ltac solve_false := try intro; solve [false; eauto with falseHd].
 
@@ -30,43 +27,63 @@ Proof.
   inverts~ H.
 Qed.
 
+#[export]
 Hint Resolve ord_and_inv toplike_int_inv toplike_arrow_inv : falseHd.
 
 
+(* topLike *)
+Lemma toplike_super_top: forall A,
+    topLike A <-> sub t_top A.
+Proof.
+  intro A.
+  split.
+  - intro H.
+    induction~ H.
+  - intro H.
+    induction~ A;
+      try solve [inverts* H].
+Qed.
+
+#[export]
+Hint Resolve toplike_super_top : core.
 
 Lemma sub_inversion_arrow : forall A1 A2 B1 B2,
-    sub (t_arrow A1 A2) (t_arrow B1 B2) -> sub t_top B2 \/ (sub B1 A1 /\ sub A2 B2).
+    sub (t_arrow A1 A2) (t_arrow B1 B2) -> topLike B2 \/ (sub B1 A1 /\ sub A2 B2).
+Proof.
+  intros.
+  inverts* H.
+  - inverts* H0.
+Qed.
+
+
+Lemma sub_inversion_arrow_r : forall A1 A2 B1 B2,
+    sub (t_arrow A1 A2) (t_arrow B1 B2) -> sub A2 B2.
+Proof.
+  intros.
+  forwards* [?|?]: sub_inversion_arrow H.
+Qed.
+
+Lemma sub_inversion_arrow_l : forall A1 A2 B1 B2,
+    ~ topLike B2 -> sub (t_arrow A1 A2) (t_arrow B1 B2) -> sub B1 A1.
+Proof.
+  intros.
+  forwards* [?|?]: sub_inversion_arrow H0.
+Qed.
+
+Lemma sub_inversion_and_l : forall A1 A2 B,
+    sub (t_and A1 A2) B -> sub A1 B \/ sub A2 B \/ exists B1 B2, B = t_and B1 B2.
 Proof.
   intros.
   inverts* H.
 Qed.
 
-Lemma sub_inversion_andl_arrr : forall A1 A2 B1 B2,
-    sub (t_and A1 A2) (t_arrow B1 B2) -> sub A1 (t_arrow B1 B2) \/ sub A2 (t_arrow B1 B2).
-Proof.
-  intros.
-  inverts* H.
-Qed.
 
-Lemma sub_inversion_toparr : forall B C,
-    sub t_top B -> sub B C -> sub t_top C.
+Lemma toplike_sub: forall A B,
+    topLike A -> sub A B -> topLike B.
 Proof.
-  intros B C S1 S2.
-  gen C.
-  remember (t_top).
-  induction S1;
-    inverts* Heqt;
-    intros C S2.
-  - intuition eauto.
-    remember (t_arrow B1 B2).
-    induction S2;
-      inverts* Heqt.
-  - intuition eauto.
-    remember (t_and A2 A3).
-    induction S2;
-      inverts* Heqt.
+  introv TL S.
+  induction S; inverts* TL.
 Qed.
-
 
 
 Lemma sub_reflexivity : forall A,
@@ -76,49 +93,31 @@ Proof.
   induction* A.
 Qed.
 
-Require Import Program.Equality.
-
-Hint Constructors sub : core.
+#[export]
+Hint Resolve sub_reflexivity : core.
 
 Lemma and_inversion : forall A B C,
     sub A (t_and B C) -> sub A B /\ sub A C.
 Proof.
   intros A B C H.
-  dependent induction H; eauto.
-  lets*: IHsub B C.
-  lets*: IHsub B C.
+  inductions H; eauto.
+  - inverts* H.
+  - lets*: IHsub B C.
+  - lets*: IHsub B C.
 Qed.
 
-Lemma sub_transtivity : forall B A,
-      sub A B -> forall C, sub B C -> sub A C.
-Proof.
-  induction B;
-    intros;
-    eauto;
-    try solve [dependent induction H0;
-               eauto].
-  - dependent induction H0; eauto.
-    clear IHsub1 IHsub2.
-    dependent induction H; eauto.
-  - apply and_inversion in H.
-    destruct H.
-    dependent induction H0; eauto.
-Qed.
-
-(* topLike *)
-Lemma toplike_super_top: forall A,
-    topLike A <-> sub t_top A.
-Proof.
-  intro A.
-  split.
-  - intro H.
-    induction H.
-    + apply sub_reflexivity.
-    + apply~ S_andr.
-    + apply~ S_toparr.
-  - intro H.
-    induction A;
-      try solve [inverts* H].
+Lemma sub_transtivity : forall B A C,
+      sub A B -> sub B C -> sub A C.
+Proof with eauto.
+  introv S1 S2. gen A C.
+  induction B; intros;
+    try solve [inductions S2; eauto].
+  - inductions S2...
+    clear IHS2_1 IHS2_2.
+    inductions S1...
+    applys S_top. applys toplike_sub H...
+  - forwards* (?&?): and_inversion S1.
+    inductions S2...
 Qed.
 
 
@@ -137,9 +136,9 @@ Ltac auto_sub :=
         try apply S_andl2;
         try apply sub_reflexivity)
       | [ H: sub t_top ?A |- sub _ ?A ] =>
-        (applys sub_transtivity H; auto)
+        (applys~ sub_transtivity H)
       | [ H: topLike ?A |- sub _ ?A ] =>
-        (apply toplike_super_top in H; applys sub_transtivity H; auto)
+        (applys~ S_top)
       | [ H: topLike ?A |- sub _ (t_arrow _ ?A) ] =>
         (apply TL_arr in H; apply S_top; auto)
       | [ H: sub (t_arrow _ _) (t_arrow _ _) |- sub _ _ ] => (apply sub_inversion_arrow in H; destruct H; auto_sub)
@@ -149,59 +148,27 @@ Ltac auto_sub :=
       end.
 
 
-Lemma toplike_sub: forall A B,
-    topLike A -> sub A B -> topLike B.
-Proof.
-  intros A B H H0.
-  apply toplike_super_top in H.
-  apply toplike_super_top.
-  auto_sub.
-Qed.
-
-
 Lemma toplike_decidable : forall A,
     topLike A \/ ~topLike A.
 Proof.
-  induction A.
-  - right.
-    unfold not.
-    intros H.
-    inversion H.
-  - left*.
-  - destruct IHA2.
-    + left*.
-    + right.
-      unfold not.
-      intros H0.
-      inverts H0.
-      auto.
-  - destruct IHA1.
-    + destruct IHA2.
-      * left*.
-      * right.
-        unfold not.
-        intros H1.
-        inverts H1.
-        auto.
-    + right.
-      unfold not.
-      intros H0.
-      inverts H0.
-      auto.
+  intros.
+  induction~ A;
+    try solve [ right; intros HF; inverts~ HF ].
+  - destruct IHA1; destruct IHA2; eauto;
+      try solve [ right; intros HF; inverts~ HF ].
+  - destruct IHA1; destruct IHA2; eauto;
+      try solve [ right; intros HF; inverts~ HF ].
 Qed.
 
-(* disjoint *)
 
+(* disjoint *)
 Lemma disjoint_eqv: forall A B,
     disjointSpec A B <-> disjoint A B.
 Proof.
-  intros A B.
-  unfold disjointSpec.
+  intros A B. unfold disjointSpec.
   split.
   - gen B.
-    induction A;
-      introv H;
-      induction B;
+    induction A; intros; induction B;
       try solve [constructor*].
     + (* int int *)
       assert (~topLike t_int). {
@@ -218,153 +185,75 @@ Proof.
       intros.
       remember (t_arrow (t_and A1 B1) C).
       assert (TL: topLike t). {
-        apply H;
-          subst;
-          constructor*;
-          [apply S_andl1 | apply S_andl2];
-          auto_sub.
+        apply H; subst*.
       }
       subst.
       inverts* TL.
-  - intros H C S1 S2.
-    apply toplike_super_top.
-    gen B C.
-    induction* A;
-      intros B H;
-      [ induction* B | induction* B | skip ];
-      intros C S1 S2;
-      try solve [inverts H].
-    + (* int arr *)
-      induction* C;
-        inverts S1;
-        inverts* S2.
-    + (* int and *)
-      induction* C;
-      inverts H;
-      inverts* S1;
-      try solve [
-        inverts S2;
-        [ forwards*: IHB1 |
-          forwards*: IHB2 ]
-          ].
-      assert (T1 : sub (t_and B1 B2) C1) by auto_sub.
-      forwards*: IHC1 T1.
-      assert (T2 : sub (t_and B1 B2) C2) by auto_sub.
-      forwards*: IHC2 T2.
-    + (* arr int *)
-      induction* C;
-        inverts S1;
-        inverts* S2.
-    + (* arr arr *)
-      inverts H.
-      induction* C;
-        inverts S1;
-        inverts* S2.
-    + (* arr and *)
-      induction* C;
-      inverts* H;
-      inverts* S1.
-      *
-        inverts S2;
-        forwards*: IHB1.
-      *
-      assert (T1 : sub (t_and B1 B2) C1) by auto_sub.
-      forwards*: IHC1 T1.
-      assert (T2 : sub (t_and B1 B2) C2) by auto_sub.
-      forwards*: IHC2 T2.
+  - intros H C S1 S2. gen C.
+    induction* H; intros; induction* C;
+      try solve [applys* toplike_super_top];
+      (* when A is an intersection type *)
+      try (forwards* [?|[?|(?&?&HF)]]: sub_inversion_and_l S1; inverts HF);
+      (* when B is an intersection type *)
+      try (forwards* [?|[?|(?&?&HF)]]: sub_inversion_and_l S2; inverts HF);
+      (* when C is an intersection type *)
+    try solve [ applys TL_and;
+                [forwards*: IHC1 | forwards*: IHC2];
+                auto_sub ];
+    (* when S1/S2 is impossible *)
+    try solve [inverts~ S1];
+    try solve [inverts~ S2].
+    (* all are arrow types *)
+    forwards* : sub_inversion_arrow_r S1.
+    forwards* : sub_inversion_arrow_r S2.
 Qed.
 
-(*
-Lemma disjoint_domain_type: forall A B C B',
-    disjointSpec (t_arrow B C) A -> disjointSpec (t_arrow B' C) A.
+
+Lemma disjoint_and_inv: forall A B C,
+    disjoint (t_and B C) A <-> disjoint B A /\ disjoint C A.
 Proof.
-  intros A B C B' H.
-  apply disjoint_eqv in H.
-  apply disjoint_eqv.
-  induction* A;
-    invert* H.
+  split; intro H.
+  - split; induction A; invert* H.
+  - destruct H; induction* A.
 Qed.
-*)
 
 
-Lemma disjoint_and: forall A B C,
+Lemma disjointSpec_and_inv: forall A B C,
     disjointSpec (t_and B C) A <-> disjointSpec B A /\ disjointSpec C A.
 Proof.
   split;
   intro H.
   - apply disjoint_eqv in H.
-    split;
-      apply disjoint_eqv;
-      induction A;
-      invert* H.
+    apply disjoint_and_inv in H.
+    split; apply disjoint_eqv; jauto.
   - destruct H.
     apply disjoint_eqv in H.
     apply disjoint_eqv in H0.
     apply disjoint_eqv.
-    induction* A.
+    applys~ disjoint_and_inv.
 Qed.
 
-
-Lemma disjoint_and2: forall A B C,
-    disjoint (t_and B C) A <-> disjoint B A /\ disjoint C A.
-Proof.
-  split;
-  intro H.
-  -
-    split;
-      induction A;
-      invert* H.
-  - destruct H.
-    induction* A.
-Qed.
-
-Lemma disjoint_symmetric: forall A B,
+Lemma disjointSpec_symmetric: forall A B,
     disjointSpec A B -> disjointSpec B A.
 Proof.
   intros A B H.
   unfold disjointSpec in H.
   unfold disjointSpec.
   intros C H0 H1.
-  forwards*: H.
+  applys~ H.
 Qed.
 
-Lemma disjoint_symmetric2: forall A B,
+Lemma disjoint_symmetric: forall A B,
     disjoint A B -> disjoint B A.
 Proof.
   intros A B H.
   apply disjoint_eqv in H.
   apply disjoint_eqv.
-  unfold disjointSpec in H.
-  unfold disjointSpec.
-  intros C H0 H1.
-  forwards*: H.
+  applys~ disjointSpec_symmetric.
 Qed.
 
 
-(* sub *)
-Lemma sub_inversion_arrow_r : forall A1 A2 B1 B2,
-    sub (t_arrow A1 A2) (t_arrow B1 B2) -> sub A2 B2.
-Proof.
-  intros.
-  apply sub_inversion_arrow in H.
-  inverts* H.
-  apply~ (sub_transtivity t_top); auto_sub.
-Qed.
-
-
-Lemma sub_inversion_arrow_l : forall A1 A2 B1 B2,
-    ~ topLike B2 -> sub (t_arrow A1 A2) (t_arrow B1 B2) -> sub B1 A1.
-Proof.
-  intros.
-  apply sub_inversion_arrow in H0.
-  inverts* H0.
-  - exfalso.
-    apply H.
-    apply toplike_super_top; auto.
-Qed.
-
-
-Lemma disjoint_domain_type: forall A B C B',
+Lemma disjointSpec_domain_type: forall A B C B',
     disjointSpec (t_arrow B C) A -> disjointSpec (t_arrow B' C) A.
 Proof.
   intros A B C B' H.
@@ -375,7 +264,7 @@ Proof.
 Qed.
 
 
-(* subsub *)
+(* Runtime Subtype *)
 Lemma subsub2sub : forall A B,
     subsub A B -> sub A B.
 Proof.
@@ -398,15 +287,12 @@ Proof.
       forwards~: IHB2.
       lets~: sub_transtivity H1 H2.
     + (* toplike *)
-      inverts H.
       apply subsub2sub in H4.
-      lets~: sub_transtivity H3 H4.
+      lets*: toplike_sub H.
   - (* and *)
     inverts~ S1; inverts~ S2; try solve_false.
-    inverts H.
     apply subsub2sub in H2. apply subsub2sub in H4.
-    forwards~: sub_transtivity H5 H2.
-    forwards~: sub_transtivity H6 H4.
+    lets*: toplike_sub H.
 Qed.
 
 
@@ -422,21 +308,21 @@ Proof.
       apply IHsubsub in H2;
       constructor*.
   - split; intro Dis;
-      apply disjoint_and2;
+      apply disjoint_and_inv;
       split;
-      apply disjoint_and2 in Dis;
+      apply disjoint_and_inv in Dis;
       destruct Dis;
       try apply IHsubsub1;
       try apply IHsubsub2;
       auto.
   - split; intros;
       apply disjoint_eqv;
-      intros T sub1 sub2;
-      apply toplike_super_top;
-      auto_sub.
+      intros T sub1 sub2.
+    applys~ toplike_sub H.
+    applys~ toplike_super_top.
 Qed.
 
-Lemma subsub_disjoint_l : forall x A B,
+Lemma subsub_disjointSpec_l : forall x A B,
     subsub x A -> disjointSpec A B -> disjointSpec x B.
 Proof.
   intros x A B H H0.
@@ -445,16 +331,16 @@ Proof.
   forwards*: disjoint_subsub2 H.
 Qed.
 
-Lemma subsub_disjoint_r : forall x A B,
+Lemma subsub_disjointSpec_r : forall x A B,
     subsub x B -> disjointSpec A B -> disjointSpec A x.
 Proof.
   intros x A B H H0.
-  apply disjoint_symmetric.
-  apply disjoint_symmetric in H0.
-  forwards*: subsub_disjoint_l H.
+  apply disjointSpec_symmetric.
+  apply disjointSpec_symmetric in H0.
+  forwards*: subsub_disjointSpec_l H.
 Qed.
 
-(* convert to arrow Type *)
+(* Applicative Distributivity: convert a type to an arrow Type *)
 Lemma arrTyp_subsub: forall A B C C',
     arrTyp C (t_arrow A B) -> subsub C' C
     -> exists A' B', arrTyp C' (t_arrow A' B') /\ sub A A' /\ subsub B' B.
@@ -462,8 +348,7 @@ Proof.
   introv Harr Hsub.
   inductions Harr.
   - inverts* Hsub.
-    * exists. repeat split*. auto_sub.
-    * exists. repeat split*. constructor. inverts* H.
+    * exists. repeat split*. inverts* H.
   - inverts* Hsub.
 Qed.
 
